

# Mathematical analysis. Lesson 10. Homework

Plyuhin Aleksandr

1

$$\begin{aligned} & \int (2x^2 - 2x - 1 + \sin x - \cos x + \ln x + e^x) dx = \\ & = 2 \int x^2 dx - 2 \int x dx - \int dx + \int \sin x dx - \int \cos x dx + \int \ln x dx + \int e^x dx = \\ & = 2 \frac{x^3}{3} - 2 \frac{x^2}{2} - x - \cos x - \sin x + x \ln x - x + e^x + C \end{aligned}$$

2

$$\begin{aligned} & \int (2x + 6xz^2 - 5x^2y - 3 \ln z) dx = \\ & = 2 \int x dx + 6z^2 \int x dx - 5y \int x^2 dx - 3 \ln z \int dx = \\ & = 2 \frac{x^2}{2} + 6z^2 \frac{x^2}{2} - 5y \frac{x^3}{3} - 3x \ln z + C \end{aligned}$$

3

$$\begin{aligned} & \int_0^\pi 3x^2 \sin(2x) dx \\ & 3 \int x^2 \sin(2x) dx = 3 \int u dv = * \\ & u = x^2, \quad du = 2x dx \\ & dv = \sin(2x) dx, \quad v = \int \sin(2x) dx = \frac{1}{2} \int \sin(2x) d(2x) = -\frac{1}{2} \cos(2x) \\ & * = 3(uv - \int v du) = 3(x^2(-\frac{1}{2} \cos(2x)) - \int (-\frac{1}{2} \cos(2x) 2x dx)) = \\ & = 3(-\frac{1}{2} x^2 \cos(2x) + \int x \cos(2x) dx) = ** \\ & \int x \cos(2x) dx = \int u dv = * \\ & u = x, \quad du = dx \\ & dv = \cos(2x) dx, \quad v = \int \cos(2x) dx = \frac{1}{2} \int \cos(2x) d(2x) = \frac{1}{2} \sin(2x) \\ & * = uv - \int v du = \frac{1}{2} x \sin(2x) - \frac{1}{2} \int \sin(2x) dx = \\ & = \frac{1}{2} x \sin(2x) - \frac{1}{2} (-\frac{1}{2} \cos(2x)) = \frac{1}{2} x \sin(2x) + \frac{1}{4} \cos(2x) \\ & ** = 3(-\frac{1}{2} x^2 \cos(2x) + \frac{1}{2} x \sin(2x) + \frac{1}{4} \cos(2x)) + C = \\ & = -\frac{3}{2} x^2 \cos(2x) + \frac{3}{2} x \sin(2x) + \frac{3}{4} \cos(2x) + C \\ & \int_0^\pi 3x^2 \sin(2x) dx = \\ & = (-\frac{3}{2} x^2 \cos(2x) + \frac{3}{2} x \sin(2x) + \frac{3}{4} \cos(2x))|_0^\pi = F(\pi) - F(0) = \\ & = -\frac{3}{2} \pi^2 \cos(2\pi) + \frac{3}{2} \pi \sin(2\pi) + \frac{3}{4} \cos(2\pi) - (\frac{3}{4} \cos 0) = \\ & = -\frac{3}{2} \pi^2 \cdot 1 + \frac{3}{2} \pi \cdot 0 + \frac{3}{4} \cdot 1 - \frac{3}{4} \cdot 1 = -\frac{3}{2} \pi^2 \end{aligned}$$

4

$$\begin{aligned} \int \frac{dx}{\sqrt{x+1}} &= * \\ t = x + 1, dt &= dx, x = t - 1 \\ * &= \int \frac{dt}{\sqrt{t-1+1}} = \int t^{-\frac{1}{2}} dt = \frac{t^{\frac{1}{2}}}{\frac{1}{2}} = 2\sqrt{t} + C = 2\sqrt{x+1} + C \end{aligned}$$